Finished SimplLocals

cfrontend/SimplLocalsproof.v
@@ -18,6 +18,8 @@ Require Import AST Linking.
 Require Import Values Memory Globalenvs Events Smallstep.
 Require Import Ctypes Cop Clight SimplLocals.
 
+Require Import Coq.Logic.FunctionalExtensionality.
+
 Module VSF := FSetFacts.Facts(VSet).
 Module VSP := FSetProperties.Properties(VSet).
 
@@ -659,12 +661,220 @@ Proof.
   exploit H2; eauto. eapply Mem.valid_block_alloc; eauto.
 Qed.
 
-Lemma match_alloc_variables:
-  forall cenv e m vars e' m',
-  alloc_variables ge e m vars e' m' ->
-  forall j tm te,
+Section SINJ.
+Definition posenv := PTree.t positive.
+Definition empty_posenv : posenv := PTree.empty positive.
+
+Fixpoint build_penv (ce:compilenv) (vars:list (ident*type)) (idx1 idx2 : positive) : posenv :=
+  match vars with
+    |nil => empty_posenv
+    |(id,ty)::l0 => if VSet.mem id ce then build_penv ce l0 (Pos.succ idx1) (idx2)
+                   else (PTree.set idx1 idx2 (build_penv ce l0 (Pos.succ idx1) (Pos.succ idx2)))
+  end.
+
+Lemma build_penv_low : forall ce vars idx1 idx2 id,
+    (id < idx1)%positive ->
+    PTree.get id (build_penv ce vars idx1 idx2) = None.
+Proof.
+  induction vars; intros; simpl. apply PTree.gempty.
+  simpl. destr. destr. apply IHvars. lia.
+  rewrite PTree.gso. apply IHvars. lia. lia.
+Qed.
+
+Definition find_func_pos (fid:ident)( pos: positive) : option positive:=
+  match Genv.find_funct_ptr ge (Global fid) with
+    |Some ((Internal f)) =>
+  let cenv := cenv_for f in
+  let penv := build_penv cenv ((f.(fn_params) ++ f.(fn_vars))) 1%positive 1%positive  in
+    PTree.get pos penv
+    |_ => None
+  end.
+
+Definition unchecked_meminj : meminj :=
+  fun b => match b with
+    |Stack (Some id) path pos =>
+      match find_func_pos id pos with
+        | Some pos' => Some(Stack (Some id) path pos',0)
+        | None => None
+      end
+    |_ => Some (b,0)
+    end.
+
+Definition struct_meminj (s:sup) : meminj :=
+  fun b => if Mem.sup_dec b s then
+           unchecked_meminj b else None.
+
+Lemma sinj_refl:
+  forall s1 s2, (forall b, sup_In b s1 <-> sup_In b s2) ->
+           struct_meminj s1= struct_meminj s2.
+Proof.
+  intros.
+  apply functional_extensionality.
+  intros. destruct x; unfold struct_meminj; simpl.
+  destruct (Mem.sup_dec (Stack f p p0) s1);
+  destruct (Mem.sup_dec (Stack f p p0) s2).
+  auto. apply H in s. congruence.
+  apply H in s. congruence. auto.
+  destr; destr. apply H in s. congruence.
+  apply H in s. congruence.
+Qed.
+
+Lemma sinj_include_incr :forall s1 s2, Mem.sup_include s1 s2 -> inject_incr (struct_meminj s1) (struct_meminj s2).
+Proof.
+  intros. intro. intros. unfold struct_meminj in *.
+  destruct b; simpl in *.
+  destruct (Mem.sup_dec (Stack f p p0) s1);
+  destruct (Mem.sup_dec (Stack f p p0) s2).
+  auto. apply H in s. congruence. inv H0. inv H0.
+  destr. destr_in H0. destr_in H0.
+  inv H0. apply H in s. congruence.
+Qed.
+
+Inductive alloc_variables' (ge:genv): env -> mem -> list (ident * type) -> list block -> env -> mem -> Prop :=
+  |av_nil : forall e m, alloc_variables' ge e m nil nil e m
+  |av_cons : forall e m id ty vars m1 b1 m2 e2 blocks,
+      Mem.alloc m 0 (sizeof ge ty) = (m1,b1) ->
+      alloc_variables' ge (PTree.set id (b1,ty) e) m1 vars blocks e2 m2 ->
+      alloc_variables' ge e m ((id,ty)::vars) (b1::blocks) e2 m2.
+
+
+Lemma alloc_vars_fresh' : forall ge e1 m1 vars blocks e2 m2 b ,
+    alloc_variables' ge e1 m1 vars blocks e2 m2 ->
+    In b blocks -> ~ sup_In b (Mem.support m1).
+Proof.
+  intros. induction H. inv H0.
+  inv H0. eapply Mem.fresh_block_alloc; eauto.
+  intro. apply IHalloc_variables'. auto.
+  eapply Mem.valid_block_alloc; eauto.
+Qed.
+
+Lemma valid_block_alloc_vars' : forall ge e1 m1 vars blocks e2 m2 b,
+    alloc_variables' ge e1 m1 vars blocks e2 m2 ->
+    sup_In b (Mem.support m1) -> sup_In b (Mem.support m2).
+Proof.
+  intros. induction H. auto.
+  eapply Mem.valid_block_alloc in H; eauto.
+Qed.
+
+Lemma alloc_vars_valid' : forall ge e1 m1 vars blocks e2 m2 b ,
+    alloc_variables' ge e1 m1 vars blocks e2 m2 ->
+    In b blocks -> sup_In b (Mem.support m2).
+Proof.
+  intros. induction H. inv H0.
+  inv H0.
+  eapply valid_block_alloc_vars' in H1; eauto.
+  eapply Mem.valid_new_block; eauto.
+  eauto.
+Qed.
+
+Lemma alloc_vars_inv'  : forall ge e1 m1 vars blocks e2 m2 b ,
+    alloc_variables' ge e1 m1 vars blocks e2 m2 ->
+    sup_In b (Mem.support m1) \/In b blocks <-> sup_In b (Mem.support m2).
+Proof.
+  intros. split. intros [A|B].
+  eapply valid_block_alloc_vars'; eauto.
+  eapply alloc_vars_valid'; eauto.
+  intros. induction H. eauto.
+  apply IHalloc_variables' in H0. inv H0.
+  destruct (eq_block b b1). right. left. auto.
+  left. exploit Mem.valid_block_alloc_inv; eauto.
+  intros. inv H0. congruence. auto. right. right. auto.
+Qed.
+
+Lemma alloc_var_var' : forall ge e1 m1 vars e2 m2,
+    alloc_variables ge e1 m1 vars e2 m2 ->
+    exists blocks, alloc_variables' ge e1 m1 vars blocks e2 m2 /\
+               list_norepet blocks.
+Proof.
+  intros. induction H.
+  exists nil. split. constructor. constructor.
+  destruct IHalloc_variables as (blocks & A & B).
+  exists (b1::blocks). split. econstructor; eauto.
+  constructor; auto. intro. apply alloc_vars_fresh' with (b:=b1)in A; auto.
+  apply A. eapply Mem.valid_new_block; eauto.
+Qed.
+
+Lemma alloc_var'_var : forall ge e1 m1 vars blocks e2 m2,
+    alloc_variables' ge e1 m1 vars blocks e2 m2 ->
+    alloc_variables ge e1 m1 vars e2 m2.
+Proof.
+  intros. induction H. constructor.
+  econstructor; eauto.
+Qed.
+
+End SINJ.
+
+Definition nextblock_pos (m:mem) (p:positive) : Prop :=
+  exists id path, Mem.nextblock m = Stack id path p.
+
+Definition match_penv_meminj (b:block) (pe:posenv) (f:meminj) : Prop :=
+  exists id path pos, b = Stack id path pos /\
+                 (f b = match pe ! pos with
+                          |Some pos' => Some ((Stack id path pos'),0)
+                          |None => None
+                 end ).
+
+Lemma nextblock_pos_succ : forall m m1 lo hi p b,
+    nextblock_pos m p ->
+    Mem.alloc m lo hi = (m1,b) ->
+    nextblock_pos m1 (Pos.succ p).
+Proof.
+  intros.
+  caseEq (Mem.alloc m1 lo hi). intros.
+  destruct H as (id & path & H). apply Mem.alloc_result in H0 as H0'. subst.
+  exploit Mem.alloc_alloc. apply H0. apply H1. eauto. intro.
+  exists id,path.
+  apply Mem.alloc_result in H1 as H1'. subst. eauto.
+Qed.
+
+Lemma nextblock_pos_1 : forall m m1 id path,
+    Mem.alloc_frame m id = (m1,path) ->
+    nextblock_pos m1 1.
+Proof.
+  intros. caseEq (Mem.alloc m1 1 1). intros.
+  exploit Mem.alloc_frame_alloc; eauto. intro.
+  apply Mem.alloc_result in H0. exists (Some id),path. congruence.
+Qed.
+
+Lemma alloc_nextblock : forall m m1 lo hi b id path p,
+    Mem.nextblock m = Stack id path p ->
+    Mem.alloc m lo hi = (m1,b) ->
+    Mem.nextblock m1 = Stack id path (Pos.succ p).
+Proof.
+  intros. caseEq (Mem.alloc m1 0 0). intros.
+  exploit Mem.alloc_alloc. apply H0. eauto.
+  apply Mem.alloc_result in H0. subst. eauto. intro.
+  apply Mem.alloc_result in H1. congruence.
+Qed.
+
+Lemma nextblock_alloc_vars :
+  forall m1 m2 ge e1 e2 vars blocks,
+    alloc_variables' ge e1 m1 vars blocks e2 m2 ->
+    forall id path p,
+    Mem.nextblock m1 = Stack id path p ->
+    (forall b, In b blocks ->
+          exists p', b = Stack id path p' /\ (p <= p')%positive).
+Proof.
+  induction 1.
+  intros. inv H0.
+  intros. inv H2.
+  - apply Mem.alloc_result in H. subst. rewrite H1.
+    exists p. split. auto. lia.
+  - exploit alloc_nextblock; eauto. intro.
+    eapply IHalloc_variables' in H2. destruct H2 as (p' & A & B).
+    exists p'. split. eauto. lia. auto.
+Qed.
+
+Lemma match_alloc_variables':
+  forall cenv e m vars blocks e' m',
+  alloc_variables' ge e m vars blocks e' m' ->
+  forall j tm te pe idx1 idx2,
   list_norepet (var_names vars) ->
   Mem.inject j m tm ->
+  Mem.stackseq m tm ->
+  pe = build_penv cenv vars idx1 idx2 ->
+  nextblock_pos m idx1 ->
+  nextblock_pos tm idx2 ->
   exists j', exists te', exists tm',
       alloc_variables tge te tm (remove_lifted cenv vars) te' tm'
   /\ Mem.inject j' m' tm'
@@ -679,24 +889,30 @@ Lemma match_alloc_variables:
        /\ if VSet.mem id cenv
           then te'!id = te!id /\ j' b = None
           else exists tb, te'!id = Some(tb, ty) /\ j' b = Some(tb, 0))
-  /\ (forall id, ~In id (var_names vars) -> e'!id = e!id /\ te'!id = te!id).
+  /\ (forall id, ~In id (var_names vars) -> e'!id = e!id /\ te'!id = te!id)
+  /\ (forall b, In b blocks -> match_penv_meminj b pe j').
 Proof.
   induction 1; intros.
   (* base case *)
   exists j; exists te; exists tm. simpl.
   split. constructor.
   split. auto. split. auto. split. auto.  split. auto.
-  split. intros. elim H2. eapply Mem.mi_mappedblocks; eauto.
-  split. tauto. auto.
+  split. intros. elim H6. eapply Mem.mi_mappedblocks; eauto.
+  split. tauto. tauto.
 
   (* inductive case *)
   simpl in H1. inv H1. simpl.
-  destruct (VSet.mem id cenv) eqn:?. simpl.
+  destruct (VSet.mem id cenv) eqn:?.
+  - simpl.
   (* variable is lifted out of memory *)
   exploit Mem.alloc_left_unmapped_inject; eauto.
   intros [j1 [A [B [C D]]]].
-  exploit IHalloc_variables; eauto. instantiate (1 := te).
-  intros [j' [te' [tm' [J [K [L [M [N [Q [O P]]]]]]]]]].
+  exploit IHalloc_variables'; eauto.
+  eapply struct_eq_trans. 2:eauto.
+  eapply struct_eq_comm. eapply Mem.alloc_stackseq; eauto.
+  eapply nextblock_pos_succ. apply H5. eauto.
+  instantiate (1 := te).
+  intros [j' [te' [tm' [J [K [L [M [N [Q [O [P R]]]]]]]]]]].
   exists j'; exists te'; exists tm'.
   split. auto.
   split. auto.
@@ -712,7 +928,7 @@ Proof.
     (* same var *)
     subst id0.
     assert (ty0 = ty).
-      destruct H1. congruence. elim H5. unfold var_names. change id with (fst (id, ty0)). apply in_map; auto.
+      destruct H1. congruence. elim H9. unfold var_names. change id with (fst (id, ty0)). apply in_map; auto.
     subst ty0.
     exploit P; eauto. intros [X Y]. rewrite Heqb. rewrite X. rewrite Y.
     exists b1. split. apply PTree.gss.
@@ -720,15 +936,28 @@ Proof.
     rewrite M. auto. eapply Mem.valid_new_block; eauto.
     (* other vars *)
     eapply O; eauto. destruct H1. congruence. auto.
-  intros. exploit (P id0). tauto. intros [X Y]. rewrite X; rewrite Y.
+  split. intros. exploit (P id0). tauto. intros [X Y]. rewrite X; rewrite Y.
     split; auto. apply PTree.gso. intuition.
-
+  intros. inv H1. unfold match_penv_meminj.
+  exploit Mem.alloc_result; eauto. intro.
+  destruct H5 as (fid & path & H5). rewrite H5 in H1.
+  exists fid,path,idx1. split. congruence.
+  rewrite M. rewrite C. rewrite build_penv_low. auto. lia.
+  eapply Mem.valid_new_block. eauto.
+  eauto.
+-
   (* variable is not lifted out of memory *)
   exploit Mem.alloc_parallel_inject.
     eauto. eauto. apply Z.le_refl. apply Z.le_refl.
   intros [j1 [tm1 [tb1 [A [B [C [D E]]]]]]].
-  exploit IHalloc_variables; eauto. instantiate (1 := PTree.set id (tb1, ty) te).
-  intros [j' [te' [tm' [J [K [L [M [N [Q [O P]]]]]]]]]].
+  exploit IHalloc_variables'; eauto.
+  eapply struct_eq_trans. eapply struct_eq_comm.
+  eapply Mem.alloc_stackseq; eauto.
+  eapply struct_eq_trans; eauto. eapply Mem.alloc_stackseq; eauto.
+  eapply nextblock_pos_succ. apply H5. eauto.
+  eapply nextblock_pos_succ. apply H6. eauto.
+  instantiate (1 := PTree.set id (tb1, ty) te).
+  intros [j' [te' [tm' [J [K [L [M [N [Q [O [P R]]]]]]]]]]].
   exists j'; exists te'; exists tm'.
   split. simpl. econstructor; eauto. rewrite comp_env_preserved; auto.
   split. auto.
@@ -738,22 +967,22 @@ Proof.
   split. intros. transitivity (j1 b). eapply N; eauto. eapply Mem.valid_block_alloc; eauto.
     destruct (eq_block b b1); auto. subst.
     assert (j' b1 = j1 b1). apply M. eapply Mem.valid_new_block; eauto.
-    rewrite H4 in H1. rewrite D in H1. inv H1. eelim Mem.fresh_block_alloc; eauto.
+    rewrite H7 in H1. rewrite D in H1. inv H1. eelim Mem.fresh_block_alloc; eauto.
   split. intros. destruct (eq_block b' tb1).
     subst b'. rewrite (N _ _ _ H1) in H1.
     destruct (eq_block b b1). subst b. rewrite D in H1; inv H1.
     exploit (P id); auto. intros [X Y]. exists id; exists ty.
     rewrite X; rewrite Y. repeat rewrite PTree.gss. auto.
-    rewrite E in H1; auto. elim H3. eapply Mem.mi_mappedblocks; eauto.
+    rewrite E in H1; auto. elim H4. eapply Mem.mi_mappedblocks; eauto.
     eapply Mem.valid_new_block; eauto.
     eapply Q; eauto. unfold Mem.valid_block in *.
-    intro. eapply Mem.valid_block_alloc_inv in H4. destruct H4. eauto.
+    intro. eapply Mem.valid_block_alloc_inv in H7. destruct H7. eauto.
     eauto. eauto.
   split. intros. destruct (ident_eq id0 id).
     (* same var *)
     subst id0.
     assert (ty0 = ty).
-      destruct H1. congruence. elim H5. unfold var_names. change id with (fst (id, ty0)). apply in_map; auto.
+      destruct H1. congruence. elim H9. unfold var_names. change id with (fst (id, ty0)). apply in_map; auto.
     subst ty0.
     exploit P; eauto. intros [X Y]. rewrite Heqb. rewrite X. rewrite Y.
     exists b1. split. apply PTree.gss.
@@ -763,8 +992,26 @@ Proof.
     (* other vars *)
     exploit (O id0 ty0). destruct H1. congruence. auto.
     rewrite PTree.gso; auto.
-  intros. exploit (P id0). tauto. intros [X Y]. rewrite X; rewrite Y.
+  split. intros. exploit (P id0). tauto. intros [X Y]. rewrite X; rewrite Y.
     split; apply PTree.gso; intuition.
+  intros. inv H1. unfold match_penv_meminj.
+  exploit Mem.alloc_result. apply H. intro.
+  exploit Mem.alloc_result. apply A. intro.
+  destruct H5 as (id0 & path0 & H5).
+  destruct H6 as (id1 & path1 & H6).
+  exploit Mem.stackseq_id_path; eauto. intros. inv H7.
+  exists id1 ,path1,idx1. split. congruence.
+  rewrite PTree.gss. rewrite M. rewrite D. rewrite H6. auto.
+  eapply Mem.valid_new_block. eauto.
+  exploit R; eauto. intros. unfold match_penv_meminj in H1.
+  destruct H1 as (id1 & path1 & pos1 & X & Y).
+  unfold match_penv_meminj. exists id1,path1,pos1. split. auto.
+  rewrite PTree.gso. eauto.
+  exploit nextblock_pos_succ. apply H5. eauto. intro.
+  assert (pos1 >= Pos.succ idx1)%positive.
+  destruct H1 as (id0 &path0 & H1).
+  exploit nextblock_alloc_vars; eauto. intros (p' & X' & Y').
+  rewrite X in X'. inv X'. lia. lia.
 Qed.
 
 Lemma alloc_variables_load:
@@ -932,10 +1179,14 @@ Proof.
 Qed.
 
 Theorem match_envs_alloc_variables:
-  forall cenv m vars e m' temps j tm,
-  alloc_variables ge empty_env m vars e m' ->
+  forall cenv m vars e m' temps j tm blocks pe idx1 idx2,
+  alloc_variables' ge empty_env m vars blocks e m' ->
   list_norepet (var_names vars) ->
   Mem.inject j m tm ->
+  Mem.stackseq m tm ->
+  pe = build_penv cenv vars idx1 idx2 ->
+  nextblock_pos m idx1 ->
+  nextblock_pos tm idx2 ->
   (forall id ty, In (id, ty) vars -> VSet.mem id cenv = true ->
                      exists chunk, access_mode ty = By_value chunk) ->
   (forall id, VSet.mem id cenv = true -> In id (var_names vars)) ->
@@ -947,11 +1198,12 @@ Theorem match_envs_alloc_variables:
   /\ inject_incr j j'
   /\ (forall b, Mem.valid_block m b -> j' b = j b)
   /\ (forall b b' delta, j' b = Some(b', delta) -> Mem.valid_block tm b' -> j' b = j b)
-  /\ (forall id ty, In (id, ty) vars -> VSet.mem id cenv = false -> exists b, te!id = Some(b, ty)).
+  /\ (forall id ty, In (id, ty) vars -> VSet.mem id cenv = false -> exists b, te!id = Some(b, ty))
+  /\ (forall b, In b blocks -> match_penv_meminj b pe j').
 Proof.
   intros.
-  exploit (match_alloc_variables cenv); eauto. instantiate (1 := empty_env).
-  intros [j' [te [tm' [A [B [C [D [E [K [F G]]]]]]]]]].
+  exploit (match_alloc_variables' cenv); eauto. instantiate (1 := empty_env).
+  intros [j' [te [tm' [A [B [C [D [E [K [F [G I]]]]]]]]]]].
   exists j'; exists te; exists tm'.
   split. auto. split; auto.
   constructor; intros.
@@ -962,11 +1214,12 @@ Proof.
   exploit F; eauto. intros [b [P R]].
   destruct (VSet.mem id cenv) eqn:?.
   (* local var, lifted *)
-  destruct R as [U V]. exploit H2; eauto. intros [chunk X].
+  destruct R as [U V]. exploit H6; eauto. intros [chunk X].
   eapply match_var_lifted with (v := Vundef) (tv := Vundef); eauto.
   rewrite U; apply PTree.gempty.
   eapply alloc_variables_initial_value; eauto.
-  red. unfold empty_env; intros. rewrite PTree.gempty in H4; congruence.
+  eapply alloc_var'_var; eauto.
+   red. unfold empty_env; intros. rewrite PTree.gempty in H8; congruence.
   apply create_undef_temps_charact with ty.
   unfold add_lifted. apply in_or_app. left.
   rewrite filter_In. auto.
@@ -988,13 +1241,14 @@ Proof.
   apply in_or_app; auto.
 
   (* injective *)
-  eapply alloc_variables_injective. eexact H.
+  eapply alloc_variables_injective.
+  eapply alloc_var'_var; eauto.
   rewrite PTree.gempty. congruence.
-  intros. rewrite PTree.gempty in H7. congruence.
+  intros. rewrite PTree.gempty in H11. congruence.
   eauto. eauto. auto.
 
   (* range *)
-  exploit alloc_variables_range. eexact H. eauto.
+  exploit alloc_variables_range. eapply alloc_var'_var. eexact H. eauto.
   rewrite PTree.gempty. intuition congruence.
 
   (* trange *)
@@ -1024,11 +1278,11 @@ Proof.
   congruence.
 
   (* incr *)
-  eapply alloc_variables_support; eauto.
+  eapply alloc_variables_support; eapply alloc_var'_var; eauto.
   eapply alloc_variables_support; eauto.
 
   (* other properties *)
-  intuition auto. edestruct F as (b & X & Y); eauto. rewrite H5 in Y.
+  intuition auto. edestruct F as (b & X & Y); eauto. rewrite H9 in Y.
   destruct Y as (tb & U & V). exists tb; auto.
 Qed.
 
@@ -1794,6 +2048,7 @@ Inductive match_states: state -> state -> Prop :=
         (MENV: match_envs j (cenv_for f) e le m lo hi te tle tlo thi)
         (MCONT: match_cont j (cenv_for f) k tk m lo tlo)
         (MINJ: Mem.inject j m tm)
+        (VINJ: j = struct_meminj (Mem.support m))
         (MSTK: Mem.stackseq m tm)
         (COMPAT: compat_cenv (addr_taken_stmt s) (cenv_for f))
         (BOUND: Mem.sup_include hi (Mem.support m))
@@ -1804,7 +2059,9 @@ Inductive match_states: state -> state -> Prop :=
       forall fd vargs k m tfd tvargs tk tm j targs tres cconv id
         (TRFD: transf_fundef fd = OK tfd)
         (MCONT: forall cenv, match_cont j cenv k tk m (Mem.support m) (Mem.support tm))
+        (FIND: Genv.find_funct_ptr ge (Global id) = Some fd)
         (MINJ: Mem.inject j m tm)
+        (VINJ: j = struct_meminj (Mem.support m))
         (MSTK: Mem.stackseq m tm)
         (AINJ: Val.inject_list j vargs tvargs)
         (FUNTY: type_of_fundef fd = Tfunction targs tres cconv)
@@ -1815,6 +2072,7 @@ Inductive match_states: state -> state -> Prop :=
       forall v k m tv tk tm j
         (MCONT: forall cenv, match_cont j cenv k tk m (Mem.support m) (Mem.support tm))
         (MINJ: Mem.inject j m tm)
+        (VINJ: j = struct_meminj (Mem.support m))
         (MSTK: Mem.stackseq m tm)
         (RINJ: Val.inject j v tv),
       match_states (Returnstate v k m)
@@ -2063,8 +2321,12 @@ Proof.
   econstructor; split.
   eapply step_Sset_debug. eauto. rewrite typeof_simpl_expr. eauto.
   econstructor; eauto with compat.
-  eapply match_envs_assign_lifted; eauto. eapply cast_val_is_casted; eauto.
+  erewrite assign_loc_support; eauto.
+  eapply match_envs_assign_lifted; eauto.
+  eapply cast_val_is_casted; eauto.
+  erewrite assign_loc_support; eauto.
   eapply match_cont_assign_loc; eauto. exploit me_range; eauto. intros [E F]. auto.
+  erewrite assign_loc_support; eauto.
   inv MV; try congruence. inv H2; try congruence. unfold Mem.storev in H3.
   eapply Mem.store_unmapped_inject; eauto. congruence.
   unfold Mem.stackseq in *. erewrite assign_loc_support; eauto.
@@ -2083,9 +2345,10 @@ Proof.
   econstructor; eauto with compat.
   eapply match_envs_invariant; eauto.
   eapply match_cont_invariant; eauto.
+  erewrite <- assign_loc_support; eauto.
   unfold Mem.stackseq in *.
-  erewrite assign_loc_support; eauto.
   rewrite (assign_loc_support _ _ _ _ _ _ _ X); eauto.
+  erewrite assign_loc_support; eauto.
   erewrite assign_loc_support; eauto.
   erewrite assign_loc_support; eauto.
 
@@ -2107,8 +2370,8 @@ Proof.
   rewrite typeof_simpl_expr. eauto.
   instantiate (1:=id).
   instantiate (1:=tvf).
-  admit. (*about sinj*)
-  eauto. eauto. eauto.
+  inv B. unfold struct_meminj in H6. destr_in H6. simpl in H6. inv H6.
+  auto. eauto. eauto. eauto.
   erewrite type_of_fundef_preserved; eauto.
   econstructor; eauto.
   intros. econstructor; eauto.
@@ -2125,7 +2388,7 @@ Proof.
   eapply match_cont_extcall; eauto.
   inv MENV. eapply Mem.sup_include_trans. eauto. eauto.
   inv MENV; eapply Mem.sup_include_trans. eauto. eauto.
-  admit. (*About external func*)
+  admit. admit. (*About external func*)
   eapply Mem.sup_include_trans; eauto. eapply external_call_support; eauto.
   eapply Mem.sup_include_trans; eauto. eapply external_call_support; eauto.
 
@@ -2186,6 +2449,8 @@ Proof.
   intro. eapply Mem.support_return_frame_1 in P'. apply P'.
   intros. erewrite Mem.load_return_frame; eauto.
   eauto. eauto. eauto.
+  eapply sinj_refl. erewrite <- free_list_support; eauto.
+  intro. eapply Mem.support_return_frame_1 in H0. apply H0.
 
 (* return some *)
   exploit eval_simpl_expr; eauto with compat. intros [tv [A B]].
@@ -2207,6 +2472,8 @@ Proof.
   intro. eapply Mem.support_return_frame_1 in P'. apply P'.
   intros. erewrite Mem.load_return_frame; eauto.
   eauto. eauto. eauto.
+  eapply sinj_refl. erewrite <- free_list_support; eauto.
+  intro. eapply Mem.support_return_frame_1 in H2. apply H2.
 
 (* skip call *)
   exploit match_envs_free_blocks; eauto. intros [tm'1 [P Q]].
@@ -2227,6 +2494,8 @@ Proof.
   intro. eapply Mem.support_return_frame_1 in P'. apply P'.
   intros. erewrite Mem.load_return_frame; eauto.
   eauto. eauto. eauto.
+  eapply sinj_refl. erewrite <- free_list_support; eauto.
+  intro. eapply Mem.support_return_frame_1 in H1. apply H1.
 
 (* switch *)
   exploit eval_simpl_expr; eauto with compat. intros [tv [A B]].
@@ -2256,7 +2525,7 @@ Proof.
 
 (* goto *)
   generalize TRF; intros TRF'. monadInv TRF'.
-  exploit (simpl_find_label j (cenv_for f) m lo tlo lbl (fn_body f) (call_cont k) x (call_cont tk)).
+  exploit (simpl_find_label (struct_meminj (Mem.support m)) (cenv_for f) m lo tlo lbl (fn_body f) (call_cont k) x (call_cont tk)).
     eauto. eapply match_cont_call_cont. eauto.
     apply compat_cenv_for.
   rewrite H. intros [ts' [tk' [A [B [C D]]]]].
@@ -2272,11 +2541,15 @@ Proof.
     unfold var_names. rewrite map_app. auto.
   exploit Mem.alloc_frame_parallel_inject; eauto.
   intros (tm' & p' & ALL & INJ).
+  exploit alloc_var_var'; eauto. intros (blocks & VARS' & H4).
+  exploit nextblock_pos_1. apply H1. intro.
+  exploit nextblock_pos_1; eauto. intro.
+  exploit Mem.alloc_frame_parallel_stackseq; eauto. intro. inv H7.
   exploit match_envs_alloc_variables; eauto.
     instantiate (1 := cenv_for_gen (addr_taken_stmt f.(fn_body)) (fn_params f ++ fn_vars f)).
-    intros. eapply cenv_for_gen_by_value; eauto. rewrite VSF.mem_iff. eexact H5.
-    intros. eapply cenv_for_gen_domain. rewrite VSF.mem_iff. eexact H4.
-  intros [j' [te [tm'' [A [B [C [D [E [F G]]]]]]]]].
+    intros. eapply cenv_for_gen_by_value; eauto. rewrite VSF.mem_iff. eexact H8.
+    intros. eapply cenv_for_gen_domain. rewrite VSF.mem_iff. eexact H7.
+  intros [j' [te [tm'' [A [B [C [D [E [F [G I]]]]]]]]]].
   assert (K: list_forall2 val_casted vargs (map snd (fn_params f))).
   { apply val_casted_list_params. unfold type_of_function in FUNTY. congruence. }
   exploit store_params_correct.
@@ -2298,8 +2571,8 @@ Proof.
   econstructor. exact Y. exact X. exact Z. eauto. simpl. eexact A. simpl. eexact Q.
   simpl. eapply star_trans. eapply step_add_debug_params. auto. eapply forall2_val_casted_inject; eauto. eexact Q.
   eapply star_trans. eexact P. eapply step_add_debug_vars.
-  unfold remove_lifted; intros. rewrite List.filter_In in H4. destruct H4.
-  apply negb_true_iff in H5. eauto.
+  unfold remove_lifted; intros. rewrite List.filter_In in H7. destruct H7.
+  apply negb_true_iff in H8. eauto.
   reflexivity. reflexivity. traceEq.
   econstructor; eauto.
   eapply match_cont_invariant with (m:= m); eauto.
@@ -2310,13 +2583,40 @@ Proof.
   eapply bind_parameters_load; eauto. intros.
   exploit alloc_variables_range. eexact H2. eauto.
   unfold empty_env. rewrite PTree.gempty. intros [?|?]. congruence.
-  red; intros; subst b'. destruct H8. congruence.
+  red; intros; subst b'. destruct H12. congruence.
   eapply alloc_variables_load; eauto.
   erewrite Mem.load_alloc_frame; eauto.
+{
+  apply functional_extensionality. intro b0.
+  destruct (Mem.sup_dec b0 (Mem.support m0)).
+  - rewrite E. unfold struct_meminj.
+    eapply Mem.support_alloc_frame_1 in H1 as SUP1.
+    apply SUP1 in s as s1.
+    eapply alloc_variables_support in s as s2; eauto.
+    erewrite <- bind_parameters_support in s2; eauto.
+    destr; destr; try congruence. auto.
+  - destruct (Mem.sup_dec b0 (Mem.support m1)).
+    + unfold struct_meminj. destr.
+      erewrite bind_parameters_support in s; eauto.
+      unfold unchecked_meminj.
+      exploit alloc_vars_inv'. apply VARS'. intro. apply H7 in s.
+      destruct s; try congruence.
+      assert (Mem.nextblock m0 = Stack (Some id) p' 1%positive).
+      eapply Mem.alloc_frame_nextblock; eauto.
+      exploit nextblock_alloc_vars; eauto.
+      intros (p'0 & X' & Y').
+      destruct H10. subst. unfold find_func_pos.
+      rewrite FIND.
+      exploit I. eauto. intro.
+      destruct H10 as (id0 & path0 & pos & X1 & Y1).
+      rewrite Y1. inv X1. auto.
+    + inv C. rewrite mi_freeblocks; eauto. unfold struct_meminj.
+      destr; try congruence.
+      erewrite bind_parameters_support in n0; eauto.
+}
   unfold Mem.stackseq in *. rewrite T.
   erewrite bind_parameters_support; eauto.
   eapply alloc_variables_parallel_stackseq; eauto.
-  eapply Mem.alloc_frame_parallel_stackseq; eauto.
   apply compat_cenv_for.
   rewrite (bind_parameters_support _ _ _ _ _ _ H3). apply Mem.sup_include_refl.
   rewrite T; auto. apply Mem.sup_include_refl.
@@ -2334,7 +2634,7 @@ Proof.
   apply Mem.sup_include_refl. apply Mem.sup_include_refl.
   eapply external_call_support; eauto.
   eapply external_call_support; eauto.
-  admit.  (*About external func*)
+  admit. admit.  (*About external func*)
 (* return *)
   specialize (MCONT (cenv_for f)). inv MCONT.
   econstructor; split.
@@ -2349,6 +2649,14 @@ Lemma initial_states_simulation:
 Proof.
   intros. inv H.
   exploit function_ptr_translated; eauto. intros [tf [A B]].
+  assert (struct_meminj (Mem.support m0) = Mem.flat_inj (Mem.support m0)).
+  apply functional_extensionality. intro x.
+  unfold struct_meminj. unfold Mem.flat_inj.
+  destruct (Mem.sup_dec x (Mem.support m0)); auto.
+  unfold unchecked_meminj. destruct x. simpl in s.
+  erewrite Genv.init_mem_stack in s; eauto.
+  destruct p. inv s. inv H4. simpl in s. destruct n; simpl in s; inv s.
+  auto.
   econstructor; split.
   econstructor.
   eapply (Genv.init_mem_transf_partial (proj1 TRANSF)). eauto.
@@ -2359,15 +2667,19 @@ Proof.
   rewrite <- H3; apply type_of_fundef_preserved; auto.
   replace (prog_main tprog) with (prog_main prog).
   econstructor; eauto.
-  intros. instantiate (1 := Mem.flat_inj (Mem.support m0)).
+  intros.
+  rewrite H.
   econstructor. instantiate (1 := Mem.support m0).
   constructor; intros.
   unfold Mem.flat_inj. apply pred_dec_true; auto.
-  unfold Mem.flat_inj in H. destruct (Mem.sup_dec b1 (Mem.support m0)); inv H. auto.
+  unfold Mem.flat_inj in H4. destruct (Mem.sup_dec b1 (Mem.support m0)); inv H4.
+  auto.
   eapply Genv.find_symbol_not_fresh; eauto.
   eapply Genv.find_funct_ptr_not_fresh; eauto.
   eapply Genv.find_var_info_not_fresh; eauto.
   apply Mem.sup_include_refl. apply Mem.sup_include_refl.
+  apply Genv.genv_vars_eq in H1. subst. auto.
+  rewrite H.
   eapply Genv.initmem_inject; eauto.
   apply struct_eq_refl.
   constructor.
